prove code_labels of REVERSE of bootstrap code
since the code in the compiler state is in reverse

bootstrap/compileCallReplStepDecScript.sml
@@ -4,7 +4,11 @@ val _ = new_theory"compileCallReplStepDec"
 val _ = Globals.max_print_depth := 15
 
 val bootstrap_lcode_def = new_definition("bootstrap_lcode_def",
-  mk_eq(``bootstrap_lcode:bc_inst list``,rand(rand(rator(rand(rand(rand(rand(rhs(concl(repl_decs_compiled)))))))))))
+  mk_eq(``bootstrap_lcode:bc_inst list``,
+        rand(rand(rator(rand(rand(rand(rand(rhs(concl(repl_decs_compiled)))))))))))
+
+val rev_bootstrap_lcode = save_thm("rev_bootstrap_lcode",
+  (RAND_CONV(REWR_CONV bootstrap_lcode_def) THENC EVAL) ``REVERSE bootstrap_lcode``)
 
 val internal_contab_def = new_definition("internal_contab_def",
   mk_eq(``internal_contab:contab``, rand(rator(rhs(concl(repl_decs_compiled))))))
@@ -25,25 +29,28 @@ val call_repl_step_dec_compiled = save_thm("call_repl_step_dec_compiled",
 
 val inst_length_def = Define`inst_length (i:bc_inst) = (0:num)` (* TODO: replace with real one *)
 
-val code_labels_ok_bootstrap_lcode =
-  ASSUME ``code_labels_ok bootstrap_lcode``
-  |> CONV_RULE(RAND_CONV(REWR_CONV bootstrap_lcode_def))
+val code_labels_ok_rev_bootstrap_lcode =
+  ASSUME ``code_labels_ok (REVERSE bootstrap_lcode)``
+  |> CONV_RULE(RAND_CONV(REWR_CONV rev_bootstrap_lcode))
 
-val code_labels_bootstrap_lcode = save_thm("code_labels_bootstrap_lcode",
-  (RAND_CONV(REWR_CONV bootstrap_lcode_def)
-   THENC code_labels_conv code_labels_ok_bootstrap_lcode (REWR_CONV inst_length_def))
-    ``code_labels inst_length bootstrap_lcode``)
+val code_labels_rev_bootstrap_lcode = save_thm("code_labels_rev_bootstrap_lcode",
+  (RAND_CONV(REWR_CONV rev_bootstrap_lcode)
+   THENC code_labels_conv code_labels_ok_rev_bootstrap_lcode (REWR_CONV inst_length_def))
+    ``code_labels inst_length (REVERSE bootstrap_lcode)``)
 
 val call_lcode_def = new_definition("call_lcode_def",
   mk_eq(``call_lcode:bc_inst list``,rand(rand(rator(rand(rhs(concl(call_repl_step_dec_compiled))))))))
 
-val code_labels_ok_call_lcode =
-  ASSUME ``code_labels_ok call_lcode``
-  |> CONV_RULE(RAND_CONV(REWR_CONV call_lcode_def))
+val rev_call_lcode = save_thm("rev_call_lcode",
+  (RAND_CONV(REWR_CONV call_lcode_def) THENC EVAL) ``REVERSE call_lcode``)
 
-val code_labels_call_lcode = save_thm("code_labels_call_lcode",
-  (RAND_CONV(REWR_CONV call_lcode_def)
-   THENC code_labels_conv code_labels_ok_call_lcode (REWR_CONV inst_length_def))
-    ``code_labels inst_length call_lcode``)
+val code_labels_ok_rev_call_lcode =
+  ASSUME ``code_labels_ok (REVERSE call_lcode)``
+  |> CONV_RULE(RAND_CONV(REWR_CONV rev_call_lcode))
+
+val code_labels_rev_call_lcode = save_thm("code_labels_rev_call_lcode",
+  (RAND_CONV(REWR_CONV rev_call_lcode)
+   THENC code_labels_conv code_labels_ok_rev_call_lcode (REWR_CONV inst_length_def))
+    ``code_labels inst_length (REVERSE call_lcode)``)
 
 val _ = export_theory()
